Simplify the tutorial.

examples/Demo.v
@@ -1,42 +1,37 @@
-(** * Tutorial
+(** * Autosubst Tutorial
 
-    In this tutorial we will use Autosubst to formalize substitutivity and
-    subject reduction in the simply typed lambda calculus. *)
+    In this tutorial we will use Autosubst to formalize the reduction relation
+    of the untyped lambda calculus and show substitutivity. *)
 
-Require Import Autosubst List.
+Require Import Autosubst.
 
 (** ** Syntax and the substitution operation
 
-    Types and terms of the simply typed lambda calculus are described by the
-    following grammar.
+    The syntax of the untyped lambda calculus is given by the following grammar.
 
-<<
-  A, B ::= * | A -> B
-  s, t ::= x | s t | \ A. s
->>
+    #
+      <div class="code" syle="width:100%">
+       <img src="ulc.png" alt="s, t ::= x | s t | \ s"/>
+      </div>
+    #
 
-    Types are either the base type, or a function type. Terms are variables,
-    applications, or abstractions. In order to generate the substitution
-    operation for terms we will add some annotations to terms. In this case we
-    will have to mark the variable and abstraction constructor with the
-    following constructs:
+    To generate the substitution operation we need an inductive type
+    corresponding to the terms above with a few annotations.
 
-    - [var] is convertible to [nat] and indicates the constructor used for
-      variables.
-    - [{bind T}] is convertible to [T] and indicates that a variable is bound in
-      the respective subterm. *)
-
-Inductive type :=
-| TBase
-| TFun  (A B : type).
+    - There must be _exactly_ one variable constructor which has a single
+      argument of type [var]. The type [var] is convertible to [nat], which is
+      used to represent de Bruijn indices.
+    - Subterms with additional bound variables must be of type [{bind term}]
+      instead of [term]. The notation [{bind T}] is convertible to [T]. *)
 
 Inductive term :=
 | TVar (x : var)
 | App  (s t : term)
-| Lam  (A : type) (s : {bind term}).
+| Lam  (s : {bind term}).
 
 (** Now we can automatically derive the substitution operations and lemmas.
     This is done by generating instances for the following typeclasses:
+
     - [VarConstr term] provides the generic variable constructor Var for term.
       It is always equivalent to the single constructor having an argument of
       type [var]. In this example, [Var] is convertible to [TVar].
@@ -53,146 +48,63 @@ Instance Subst_term : Subst term. derive. Defined.
 Instance SubstLemmas_term : SubstLemmas term. derive. Qed.
 
 (** At this point we can use the notations:
-    - [s.[sigma]] for the application of the substitution sigma to a term s.
+
+    - [s.[sigma]] for the application of the substitution [sigma] to a term [s].
     - [sigma >> tau] for the composition of sigma and tau, i.e., the
       substitution [fun x => (sigma x).[tau]].
 
-    SubstLemmas contains the following lemmas:
-    - id_subst s x : [(Var x).[sigma] = sigma x]
-    - subst_id s : [s.[Var] = s]
-    - subst_comp sigma tau : [s.[sigma].[tau] = s.[sigma >> tau]]
-    - rename_subst xi s : [rename xi s = s.[ren xi]]
-    where [ren xi x = Var (xi x)].
-
-    In addition these lemmas allow you to use the autosubst tactic. *)
+    Additionally there is a generic cast [ren] from renamings (functions of type
+    [nat -> nat] to substitutions). Use [autosubst] to simplify terms containing
+    substitutions. *)
 
 (** ** Reduction and substitutivity
 
-    Reductions are defined by the following inference rules:
+    The single-step reduction relation is defined by the following inference
+    rules
 
-<<
-    s1 \rhd s2        t1 \rhd t2          s1 \rhd s2
-  --------------    --------------    ------------------
-  s1 t \rhd s2 t    s t1 \rhd s t2    \A. s1 \rhd \A. s2
+    #
+      <div class="code" style="text-align:center; width:100%">
+        <img src="red1.png" alt="AppL"/>
+        <img src="red2.png" alt="AppR"/>
+        <img src="red3.png" alt="Lam"/> <br/>
+        <img src="red4.png" alt="Beta"/>
+      </div>
+    #
 
-
-  ---------------------------
-  (\A. s) t \rhd s.[beta t]
->>
-
-    Where [beta t] is notation for the substitution [t .: Var].
+    The Coq notation for stream cons is [.:] and the identity substitution is
+    [Var]. Additionally, we define the abbreviation [ beta t = t .: Var ].
 
     The definition below is an almost verbatim copy of the inference rules. The
     one difference is in the beta rule. Instead of using [s.[beta t]]
     directly, we add an equation to the premise.
 
-<<
-   s2 = s1.[beta t]
-  ------------------
-  (\A. s1) t \rhd s2
->>
-
-    This makes the constructor applicable even if the substitution on [s] is not
-    of to the special form [t .: Var]. *)
+    This makes the constructor applicable even if the substitution on [s] is
+    not of to the special form [beta t]. The resulting equation can then be
+    solved using [autosubst]. *)
 
 Inductive step : term -> term -> Prop :=
-| Step_Beta (A : type) (s1 s2 t : term) :
-    s2 = s1.[beta t] -> step (App (Lam A s1) t) s2
-| Step_App1 (s1 s2 t : term) :
+| step_beta (s1 s2 t : term) :
+    s2 = s1.[beta t] -> step (App (Lam s1) t) s2
+| step_appL (s1 s2 t : term) :
     step s1 s2 -> step (App s1 t) (App s2 t)
-| Step_App2 (s t1 t2 : term) :
+| step_appR (s t1 t2 : term) :
     step t1 t2 -> step (App s t1) (App s t2)
-| Step_Lam (A : type) (s1 s2 : term) :
-    step s1 s2 -> step (Lam A s1) (Lam A s2).
+| step_lam  (s1 s2 : term) :
+    step s1 s2 -> step (Lam s1) (Lam s2).
 
-Lemma step_subst s1 s2 :
+(** The proof of substitutivity proceeds by induction on the reduction relation.
+    In every case we use [autosubst] to simplify the substitution operation and
+    apply a constructor. Apart from [step_beta] every case is trivial and solved
+    by the tactic of the same name.
+
+    In the case of beta reduction we have to show the equation
+    [s1.[t .: Var].[sigma] = s1.[up sigma].[t.[sigma] .: Var]].
+
+    This goal can be solved using [autosubst], since both sides of the equation
+    are equivalent to the normal form [s1.[t.[sigma] .: sigma]]. *)    
+
+Lemma substitutivity s1 s2 :
   step s1 s2 -> forall sigma, step s1.[sigma] s2.[sigma].
 Proof.
-(* The proof of substitutivity proceeds by induction on the step relation.
-    Every case, except for [Step_Beta] is trivial and solved by eauto. *)
-  induction 1; eauto using step.
-(* In the beta case we can apply the constructor and simplify the goal. *)
-  intros sigma. autosubst. constructor. subst.
-(* At this point our goal is to show the equation:
-<<
-   s1.[beta t].[sigma] = s1.[up sigma].[beta t.[sigma]]
->>
-    This is a parallel variant of Barendregt's famous substitution lemma.
-    As it is simply an equations between terms with substitutions we can solve
-    this goal using autosubst. In this particular case, the equation holds
-    because both sides are equivalent to the normal form
-    [s1.[t.[sigma] .: sigma]]. *)
-  now autosubst.
-Qed.
-
-(** ** Type preservation
-
-    The typing relation is defined by the following inference rules.
-
-<<
-   Gamma x = A      Gamma |- s : A -> B    Gamma |- t : A
-  --------------   ---------------------------------------
-  Gamma |- x : A             Gamma |- s t : B
-
-      Gamma, A |- s : B
-  -------------------------
-   Gamma |- \A. s : A -> B
->>
-
-    We implement contexts as lists and write [A :: Gamma] instead of "Gamma, A".
-    Apart from this, we also need to implement the "Gamma x = A" line in the
-    variable rule. Since this is just a list lookup we use the [nth_error]
-    function from the list library. *)
-
-Inductive ty (Gamma : list type) : term -> type -> Prop :=
-| Ty_Var (x : var) (A : type) :
-    nth_error Gamma x = value A -> ty Gamma (Var x) A
-| Ty_App (A B : type) (s t : term) :
-    ty Gamma s (TFun A B) -> ty Gamma t A -> ty Gamma (App s t) B
-| Ty_Lam (A B : type) (s : term) :
-    ty (A :: Gamma) s B -> ty Gamma (Lam A s) (TFun A B).
-
-(** Our goal for the rest of the tutorial is to show type preservation, that is:
-<<
-  Gamma |- s : A -> s \rhd t -> Gamma |- t : A
->>
-    As usual, this requires a substitution lemma, which in turn requires
-    weakening. Using parallel substitutions we can show a general lemma for
-    arbitrary substitutions. The weakening lemma is the special case of a
-    renaming substitution. *)
-
-Lemma ty_weak Gamma s A :
-  ty Gamma s A -> forall Delta xi,
-  (forall x B,
-     nth_error Gamma x = value B -> nth_error Delta (xi x) = value B) ->
-  ty Delta s.[ren xi] A.
-Proof.
-  induction 1; intros; autosubst; eauto using ty.
-  constructor. apply IHty. intros [|]; simpl; eauto.
-Qed.
-
-Lemma ty_subst Gamma s A :
-  ty Gamma s A -> forall Delta sigma,
-  (forall x B, nth_error Gamma x = value B -> ty Delta (sigma x) B) ->
-  ty Delta s.[sigma] A.
-Proof.
-  induction 1; intros; autosubst; eauto using ty.
-  constructor. apply IHty. intros [|]; simpl; eauto using ty, ty_weak.
-Qed.
-
-Lemma substitution Gamma s t A B :
-  ty (A :: Gamma) s B ->
-  ty Gamma t A ->
-  ty Gamma s.[beta t] B.
-Proof.
-  intros T1 T2. apply (ty_subst _ _ _ T1). intros [|x] C; simpl; eauto using ty.
-  intros H. inversion H; subst; auto.
-Qed.
-
-Lemma preservation s t :
-  step s t -> forall Gamma A, ty Gamma s A -> ty Gamma t A.
-Proof.
-  induction 1 as [A' s1 s2 t e|s1 s2 t _ ih|s t1 t2 _ ih|A s1 s2 _ ih];
-    intros Gamma B T; inversion_clear T; eauto using ty; subst.
-  inversion_clear H. revert H1 H0. apply substitution.
+  induction 1; intros; autosubst; constructor; trivial. subst. autosubst.
 Qed.
